Prove properties of avl_remove

AVLTree.v
@@ -117,6 +117,15 @@ Section Invariants.
       intuition eauto.
   Qed.
 
+  Theorem all_keys_greater_chain_eq :
+    forall (k k':N) (t:avl_tree T),
+      k' <= k -> forall_keys (N.lt k) t -> forall_keys (N.lt k') t.
+  Proof.
+    Hint Resolve N.le_lt_trans.
+    intros k k' t ineq H.
+    induction t as [b l IH [k'' v] r IHr|]; simpl in *; intuition eauto.
+  Qed.
+
   Lemma invert_tuple_eq :
     forall (A B:Type) (a a':A) (b b':B),
       (a,b) = (a',b') <-> a = a' /\ b = b'.
@@ -503,33 +512,220 @@ End Insert.
 Section Remove.
   Variable T : Type.
 
-  Fixpoint avl_remove_minimum_go (b:sign) (l:avl_tree T) (p:N * T) (r:avl_tree T)
-  : (N * T) * (avl_tree T * sign) :=
-    match l with
-      | avl_empty => (p, (r, negative))
-      | avl_branch lb ll lp lr =>
-        match avl_remove_minimum_go lb ll lp lr with
-          | (pm, (l', s)) => (pm, node b (inl s) l' p r)
-        end
+  Fixpoint avl_find_minimum (t:avl_tree T) (def:N * T): (N * T) :=
+    match t with
+      | avl_empty => def
+      | avl_branch lb ll lp lr => avl_find_minimum ll lp
     end.
 
-  Example avl_remove_minimum_go_ex1 :
+  Example avl_find_minimum_ex1 :
     forall a b c d : T,
-      avl_remove_minimum_go
-        negative
-        (avl_branch zero avl_empty (1,a) avl_empty)
-        (2,b)
-        (avl_branch positive
-                    (avl_branch zero avl_empty (3,c) avl_empty)
-                    (4,d)
-                    avl_empty) =
-      ((1,a), (avl_branch
-                 zero
-                 (avl_branch zero avl_empty (2,b) avl_empty)
-                 (3,c)
-                 (avl_branch zero avl_empty (4,d) avl_empty)
-               , negative)).
+      avl_find_minimum
+        (avl_insert 1 a (avl_insert 2 b (avl_insert 3 c (avl_insert 4 d avl_empty))))
+        (5,d)
+      = (1,a).
   Proof. intros. reflexivity. Qed.
+
+  Theorem avl_find_minimum_In :
+    forall (t:avl_tree T) (def:N * T),
+      In (avl_find_minimum t def) t \/ avl_find_minimum t def = def.
+  Proof.
+    intros t. induction t as [b l IHl p r IHr|].
+    - intros def. clear IHr. specialize IHl with p. simpl in *. intuition eauto.
+    - intros. simpl. tauto.
+  Qed.
+
+  Theorem avl_find_minimum_is_min :
+    forall (t:avl_tree T) (def:N * T),
+      binary_tree_invariant t ->
+      forall_keys (N.le (fst (avl_find_minimum t def))) t.
+  Proof.
+    Hint Resolve N.gt_lt N.lt_le_incl.
+    intros t def bt_inv. generalize dependent def. induction t as [b l IHl p r IHr|].
+    - intros def. clear IHr. simpl. specialize IHl with p. destruct p as [k v].
+      simpl in *.
+      assert (min_le_k: fst (avl_find_minimum l (k,v)) <= k).
+      {
+        destruct avl_find_minimum_In with (t := l) (def := (k,v)) as [H|H].
+        - rewrite_all forall_keys_In_iff. intuition eauto.
+        - rewrite H. reflexivity.
+      }
+      repeat split.
+      + auto.
+      + intuition auto.
+      + rewrite_all forall_keys_In_iff. intros p in_r.
+        rewrite min_le_k. apply N.lt_le_incl. intuition eauto.
+    - simpl. auto.
+  Qed.
+
+  Fixpoint avl_remove_minimum (b:sign) (l:avl_tree T) (p:N * T) (r:avl_tree T)
+  : (avl_tree T * sign) :=
+    match l with
+      | avl_empty => (r, negative)
+      | avl_branch lb ll lp lr =>
+        let (l',s) := avl_remove_minimum lb ll lp lr
+        in node b (inl s) l' p r
+    end.
+
+  Theorem avl_remove_minimum_preserve_other :
+    forall (l:avl_tree T) (p':N * T) (b:sign) (p:N * T) (r:avl_tree T),
+      p' = p \/ In p' l \/ In p' r <->
+      (In p' (fst (avl_remove_minimum b l p r)) \/ p' = avl_find_minimum l p).
+  Proof.
+    intros l p'. induction l as [lb ll IHll lp lr IHlr|].
+    - intros b p r. simpl in *.
+      destruct (avl_remove_minimum lb ll lp lr) as [l' s] eqn:rec_eq.
+      rewrite <- node_same_elements.
+      assert (l'_eq: l' = fst (l', s)) by reflexivity. rewrite <- rec_eq in l'_eq.
+      subst l'. rewrite IHll with (b := lb). tauto.
+    - intros. simpl. tauto.
+  Qed.
+
+  Theorem avl_remove_minimum_subset :
+    forall (l:avl_tree T) (p':N * T) (b:sign) (p:N * T) (r:avl_tree T),
+      In p' (fst (avl_remove_minimum b l p r)) -> p' = p \/ In p' l \/ In p' r.
+  Proof.
+    intros l p'. induction l as [lb ll IHll lp lr IHlr|].
+    - intros b p r. clear IHlr. specialize IHll with lb lp lr. simpl in *.
+      destruct (avl_remove_minimum lb ll lp lr) as [l' s] eqn:rec_eq.
+      replace l' with (fst (l',s)) by reflexivity.
+      rewrite <- node_same_elements. intuition auto.
+    - intros. simpl. auto.
+  Qed.
+
+  Theorem avl_remove_preserve_forall :
+    forall (P:N -> Prop) (b:sign) (l:avl_tree T) (p:N * T) (r:avl_tree T),
+      P (fst p) /\ forall_keys P l /\ forall_keys P r ->
+      forall_keys P (fst (avl_remove_minimum b l p r)).
+  Proof.
+    Hint Resolve avl_remove_minimum_subset.
+    intros. rewrite_all forall_keys_In_iff. intros p' in_rm.
+    apply avl_remove_minimum_subset in in_rm. intuition (subst; eauto).
+  Qed.
+
+  Theorem avl_remove_minimum_binary_tree_invariant:
+    forall (l:avl_tree T) (b:sign) (p:N * T) (r:avl_tree T),
+      binary_tree_invariant (avl_branch b l p r) ->
+      binary_tree_invariant (fst (avl_remove_minimum b l p r)).
+  Proof.
+    Hint Resolve node_binary_tree_invariant avl_remove_preserve_forall.
+    intros l. induction l as [lb ll IHll lp lr IHlr|].
+    - intros b p r bt_inv. simpl in *. clear IHlr. specialize IHll with lb lp lr.
+      simpl in *. destruct p as [k v]. destruct lp as [lk lv].
+      destruct (avl_remove_minimum lb ll (lk,lv) lr) as [l' s] eqn:min_eq.
+      replace l' with (fst (l',s)) by reflexivity. rewrite_all <- min_eq.
+      intuition eauto.
+    - intros b [k v] r. simpl in *. tauto.
+  Qed.
+
+  Theorem avl_remove_minimum_min_not_In :
+    forall (l:avl_tree T) (b:sign) (p:N * T) (r:avl_tree T),
+      binary_tree_invariant (avl_branch b l p r) ->
+      ~In (avl_find_minimum l p) (fst (avl_remove_minimum b l p r)).
+  Proof.
+    Hint Resolve N.gt_lt.
+    intros l. induction l as [lb ll IHll lp lr IHlr|].
+    - intros b p r bt_inv H. simpl in *.
+      destruct (avl_remove_minimum lb ll lp lr) as [l' s] eqn:rec_eq.
+      rewrite <- node_same_elements in H. specialize IHll with lb lp lr.
+      clear IHlr. replace l' with (fst (l', s)) in H by reflexivity.
+      rewrite_all <- rec_eq. rewrite_all forall_keys_In_iff. destruct H as [H|[H|H]].
+      + destruct avl_find_minimum_In with (t := ll) (def := lp) as [P|P].
+        * apply N.lt_irrefl with (x := fst p). subst. intuition eauto.
+        * apply N.lt_irrefl with (x := fst p). rewrite_all P. subst. intuition auto.
+      + apply IHll; intuition eauto.
+      + destruct avl_find_minimum_In with (t := ll) (def := lp) as [P|P].
+        * apply N.lt_asymm with (n := fst p) (m := fst (avl_find_minimum ll lp));
+            intuition eauto.
+        * rewrite_all P. apply N.lt_asymm with (n := fst lp) (m := fst p);
+            intuition eauto.
+    - intros b p r inv_bt H. simpl in *. rewrite_all forall_keys_In_iff.
+      apply N.lt_irrefl with (x := fst p). intuition eauto.
+  Qed.
+
+  Theorem avl_remove_minimum_removes_minimum :
+    forall (l:avl_tree T) (min_k:N) (b:sign) (p:N * T) (r:avl_tree T),
+      binary_tree_invariant (avl_branch b l p r) ->
+      forall_keys (N.le min_k) (avl_branch b l p r) ->
+      forall_keys (N.lt min_k) (fst (avl_remove_minimum b l p r)).
+  Proof.
+    Hint Resolve all_keys_greater_chain_eq all_keys_greater_chain N.le_lt_trans
+         node_preserve_forall.
+    intros l min_k. induction l as [lb ll IHll lp lr IHlr|].
+    - intros b p r bt_inv H. simpl in *. clear IHlr. specialize IHll with lb lp lr.
+      destruct (avl_remove_minimum lb ll lp lr) as [l' s] eqn:rec_eq.
+      replace l' with (fst (l', s)) by reflexivity. rewrite_all <- rec_eq.
+      intuition eauto.
+    - intros. simpl in *. intuition eauto.
+  Qed.
+
+  Theorem avl_remove_minimum_all_greater :
+    forall (l:avl_tree T) (b:sign) (p:N * T) (r:avl_tree T),
+      binary_tree_invariant (avl_branch b l p r) ->
+      forall_keys (N.lt (fst (avl_find_minimum l p))) (fst (avl_remove_minimum b l p r)).
+  Proof.
+    intros l b p r bt_inv. apply avl_remove_minimum_removes_minimum.
+    - assumption.
+    - simpl.
+      destruct avl_find_minimum_In with (t := l) (def := p) as [H|H].
+      + simpl in *. repeat split.
+        * rewrite_all forall_keys_In_iff. intuition eauto.
+        * apply avl_find_minimum_is_min. tauto.
+        * rewrite_all forall_keys_In_iff.
+          assert (pk_gt: fst (avl_find_minimum l p) <= fst p) by intuition eauto.
+          intros p' in_r.
+          assert (p'_gt: fst p < fst p') by intuition auto.
+          eapply N.le_lt_trans in p'_gt; eauto.
+      + simpl in *. rewrite_all H. repeat split.
+        * reflexivity.
+        * rewrite <- H. apply avl_find_minimum_is_min. tauto.
+        * rewrite_all forall_keys_In_iff. intros p' in_r. apply N.lt_le_incl.
+          intuition eauto.
+  Qed.
+
+
+  Definition avl_remove_top (b:sign) (l:avl_tree T) (r:avl_tree T) : avl_tree T * sign :=
+    match r with
+      | avl_empty => (l, negative)
+      | avl_branch rb rl rp rr =>
+        let (r',s) := avl_remove_minimum rb rl rp rr
+        in node b (inr s) l (avl_find_minimum rl rp) r'
+    end.
+
+  Theorem avl_remove_top_preserve_other :
+    forall (b:sign) (l:avl_tree T) (r:avl_tree T) (p:N * T),
+      (In p r \/ In p l) <-> In p (fst (avl_remove_top b l r)).
+  Proof.
+    intros b l r p. destruct r as [rb rl rp rr|] eqn:r_eq.
+    - simpl. destruct (avl_remove_minimum rb rl rp rr) as [r' s] eqn:rm_min_eq.
+      replace r' with (fst (r',s)) by reflexivity. rewrite <- rm_min_eq.
+      rewrite <- node_same_elements.
+      rewrite avl_remove_minimum_preserve_other with (b := rb).
+      tauto.
+    - subst. simpl. tauto.
+  Qed.
+
+  Theorem avl_remove_top_binary_tree_invariant :
+    forall (b:sign) (l:avl_tree T) (r:avl_tree T) (k:N),
+      forall_keys (N.gt k) l -> forall_keys (N.lt k) r ->
+      binary_tree_invariant l -> binary_tree_invariant r ->
+      binary_tree_invariant (fst (avl_remove_top b l r)).
+  Proof.
+    Hint Resolve node_binary_tree_invariant avl_remove_minimum_binary_tree_invariant
+      avl_remove_minimum_subset.
+    intros b l r k k_gt_l k_lt_r bt_inv_l bt_inv_r. destruct r as [rb rl rp rr|].
+    - simpl in *. destruct (avl_remove_minimum rb rl rp rr) as [r' s] eqn:rm_min_eq.
+      replace r' with (fst (r', s)) by reflexivity. rewrite_all <- rm_min_eq.
+      apply node_binary_tree_invariant.
+      + intuition auto.
+      + apply avl_remove_minimum_binary_tree_invariant. simpl. intuition auto.
+      + destruct avl_find_minimum_In with rl rp as [H|H].
+        * rewrite_all forall_keys_In_iff. intros p' in_l.
+          apply N.lt_gt. apply N.lt_trans with k; intuition eauto.
+        * rewrite H. apply all_keys_smaller_chain with k; intuition eauto.
+      + apply avl_remove_minimum_all_greater. simpl. intuition eauto.
+    - simpl in *. auto.
+  Qed.
 
   Fixpoint avl_remove_go (k:N) (t:avl_tree T) : avl_tree T * sign :=
     match t with
@@ -538,13 +734,7 @@ Section Remove.
         match N.compare k k' with
           | Lt => let (l',s) := avl_remove_go k l in node b (inl s) l' (k',v') r
           | Gt => let (r',s) := avl_remove_go k r in node b (inr s) l (k',v') r'
-          | Eq =>
-            match r with
-              | avl_empty => (l, negative)
-              | avl_branch rb rl rp rr =>
-                let '(p', (r',s)) := avl_remove_minimum_go rb rl rp rr in
-                node b (inr s) l p' r'
-            end
+          | Eq => avl_remove_top b l r
         end
     end.
 
@@ -591,7 +781,83 @@ Section Remove.
           (6,f)
           (avl_branch negative avl_empty (7,g) (avl_singleton 8 h)).
   Proof. reflexivity. Qed.
-End Remove.
+
+  Theorem remove_not_In :
+    forall k v t,
+      binary_tree_invariant t ->
+      ~In (k,v) (avl_remove k t).
+  Proof.
+    intros k v t bt_inv_t. induction t as [b l IHl p r IHr|].
+    - unfold avl_remove. simpl. destruct p as [k' v'] eqn:peq.
+      destruct (N.compare_spec k k') as [C|C|C].
+      + intros H. rewrite <- avl_remove_top_preserve_other in H. simpl in *.
+        rewrite_all forall_keys_In_iff. subst k. apply N.lt_irrefl with k'.
+        replace k' with (fst (k', v)) by reflexivity. intuition eauto.
+      + destruct (avl_remove_go k l) as [l' s] eqn:rec_eq.
+        replace l' with (fst (l', s)) by reflexivity.
+        rewrite <- rec_eq. unfold avl_remove in *. rewrite <- node_same_elements.
+        rewrite invert_tuple_eq. intros H. unfold not in *. simpl in *.
+        rewrite_all forall_keys_In_iff.
+        intuition (subst; (eapply N.lt_irrefl; eauto) || eauto).
+      + destruct (avl_remove_go k r) as [r' s] eqn:rec_eq.
+        replace r' with (fst (r',s)) by reflexivity.
+        rewrite <- rec_eq. unfold avl_remove in *. rewrite <- node_same_elements.
+        rewrite invert_tuple_eq. intros H. unfold not in *. simpl in *.
+        rewrite_all forall_keys_In_iff.
+        intuition (subst; (eapply N.lt_irrefl; eauto) || eauto).
+    - simpl. auto.
+  Qed.
+
+  Theorem remove_preserve_other :
+    forall (p:N * T) (k:N) (t:avl_tree T),
+      (In p t <-> (In p (avl_remove k t) \/ (fst p = k /\ In p t))).
+  Proof.
+    intros. unfold avl_remove. induction t as [b l IHl [k' v'] r IHr|].
+    - simpl. destruct (N.compare_spec k k') as [C|C|C].
+      + rewrite <- avl_remove_top_preserve_other.
+        split; intuition (subst; auto).
+      + destruct (avl_remove_go k l) as [l' s] eqn:rec_eq.
+        rewrite <- node_same_elements. replace l' with (fst (l', s)) by reflexivity.
+        rewrite IHl. tauto.
+      + destruct (avl_remove_go k r) as [r' s] eqn:rec_eq.
+        rewrite <- node_same_elements. replace r' with (fst (r', s)) by reflexivity.
+        rewrite IHr. tauto.
+    - simpl. tauto.
+  Qed.
+
+  Theorem remove_subset :
+    forall (p:N * T) (k:N) (t:avl_tree T),
+      In p (avl_remove k t) -> In p t.
+  Proof.
+    intros. rewrite remove_preserve_other with (k := k). tauto.
+  Qed.
+
+  Theorem remove_preserve_forall :
+    forall (P:N -> Prop) (k:N) (t:avl_tree T),
+      forall_keys P t -> forall_keys P (avl_remove k t).
+  Proof.
+    Hint Resolve remove_subset.
+    intros P k t H. rewrite_all forall_keys_In_iff. intros p in_rm.
+    eauto.
+  Qed.
+
+  Theorem remove_binary_tree_invariant :
+    forall (k:N) (t:avl_tree T),
+      binary_tree_invariant t -> binary_tree_invariant (avl_remove k t).
+  Proof.
+    Hint Resolve avl_remove_top_binary_tree_invariant node_binary_tree_invariant
+         remove_preserve_forall.
+    intros k t bt_inv. unfold avl_remove. induction t as [b l IHl [k' v'] r IHr|].
+    - simpl. destruct (N.compare_spec k k') as [C|C|C].
+      + subst k'. simpl in *. intuition eauto.
+      + destruct (avl_remove_go k l) as [l' s] eqn:rec_eq.
+        replace l' with (fst (l', s)) by reflexivity. rewrite_all <- rec_eq.
+        simpl in *. fold (avl_remove k l) in *. intuition eauto.
+      + destruct (avl_remove_go k r) as [r' s] eqn:rec_eq.
+        replace r' with (fst (r', s)) by reflexivity. rewrite_all <- rec_eq.
+        simpl in *. fold (avl_remove k r) in *. intuition eauto.
+    - simpl. constructor.
+  Qed.
 
 Section Lookup.
 
